src/SemanticsNew.v
@@ -1,4 +1,4 @@
-Require Import Lib.FnMap Lib.Struct.
+Require Import Lib.FMap Lib.Struct.
 Require Import Syntax Semantics Refinement.
 
 Require Import String List.
@@ -8,12 +8,12 @@ Definition bothNotRule (rm1 rm2 : bool) : Prop :=
 
 Inductive CanCombine : (RegsT * LabelT) -> (RegsT * LabelT) -> Prop :=
   MkCanCombine : forall u1 rm1 ds1 cs1 u2 rm2 ds2 cs2,
-    Disj u1 u2 -> Disj ds1 ds2 -> Disj cs1 cs2 -> bothNotRule rm1 rm2
+    MF.Disj u1 u2 -> MF.Disj ds1 ds2 -> MF.Disj cs1 cs2 -> bothNotRule rm1 rm2
    -> CanCombine (u1, (rm1, ds1, cs1)) (u2, (rm2, ds2, cs2)).
 
 Definition mergeLabel (l1 l2 : LabelT) : LabelT := match l1, l2 with
   (rm1, ds1, cs1), (rm2, ds2, cs2) =>
-    (orb rm1 rm2, union ds1 ds2, union cs1 cs2)
+    (orb rm1 rm2, MF.union ds1 ds2, MF.union cs1 cs2)
   end.
 
 Definition equivalent (l1 l2 : LabelT) (p : LabelT -> LabelT) :=
@@ -28,9 +28,9 @@ Inductive UnitStep : Modules -> RegsT -> RegsT -> LabelT -> Type :=
    (meths : list DefMethT)
    (oRegs : RegsT)
    (ruleMeth : bool),
-   InDomain oRegs (namesOf regInits)
-   -> UnitStep (Mod regInits rules meths) oRegs empty
-        (ruleMeth, empty, empty)
+   MF.InDomain oRegs (namesOf regInits)
+   -> UnitStep (Mod regInits rules meths) oRegs (M.empty _)
+        (ruleMeth, M.empty _, M.empty _)
 | SingleRule : 
   forall (ruleName : string) (ruleBody : Action (Bit 0))
    (regInits : list RegInitT)
@@ -40,9 +40,9 @@ Inductive UnitStep : Modules -> RegsT -> RegsT -> LabelT -> Type :=
   forall (oRegs news : RegsT) (calls : CallsT)
   (retV : type (Bit 0)),
   SemAction oRegs (ruleBody type) news calls retV ->
-   InDomain oRegs (namesOf regInits) ->
+   MF.InDomain oRegs (namesOf regInits) ->
   UnitStep (Mod regInits rules meths) oRegs news
-       (true, empty, calls)
+       (true, M.empty _, calls)
 | SingleMeth : forall 
    (regInits : list RegInitT)
    (rules : list (Attribute (Action Void)))
@@ -54,25 +54,25 @@ Inductive UnitStep : Modules -> RegsT -> RegsT -> LabelT -> Type :=
    (retV : type (ret (objType (attrType meth))))
    (udefs : CallsT),
    SemAction oRegs (objVal (attrType meth) type argV) news calls retV ->
-   udefs = add meth {|
+   udefs = M.add meth {|
                  objType := objType (attrType meth);
-                 objVal := (argV, retV) |} empty ->
-   InDomain oRegs (namesOf regInits) ->
+                 objVal := (argV, retV) |} (M.empty _) ->
+   MF.InDomain oRegs (namesOf regInits) ->
    UnitStep (Mod regInits rules meths) oRegs news
       (false, udefs, calls)
 | LeftIntro : forall (m1 m2 : Modules)
     (oRegs1 oRegs2 oRegs news : RegsT)
     (l : LabelT),
-    InDomain oRegs2 (namesOf (getRegInits m2)) ->
+    MF.InDomain oRegs2 (namesOf (getRegInits m2)) ->
     UnitStep m1 oRegs1 news l ->
-    oRegs = union oRegs1 oRegs2 ->
+    oRegs = MF.union oRegs1 oRegs2 ->
     UnitStep (ConcatMod m1 m2) oRegs news l
 | RightIntro : forall (m1 m2 : Modules)
     (oRegs1 oRegs2 oRegs news : RegsT)
     (l : LabelT),
-    InDomain oRegs1 (namesOf (getRegInits m1)) ->
+    MF.InDomain oRegs1 (namesOf (getRegInits m1)) ->
     UnitStep m2 oRegs2 news l ->
-    oRegs = union oRegs1 oRegs2 ->
+    oRegs = MF.union oRegs1 oRegs2 ->
     UnitStep (ConcatMod m1 m2) oRegs news l.
 
 Inductive UnitSteps (m : Modules) (o : RegsT) : RegsT -> LabelT -> Type :=
@@ -80,16 +80,16 @@ Inductive UnitSteps (m : Modules) (o : RegsT) : RegsT -> LabelT -> Type :=
  | UnitStepsUnion : forall {u1 u2 : RegsT} {l1 l2 : LabelT}, 
     UnitSteps m o u1 l1 -> UnitSteps m o u2 l2 
     -> CanCombine (u1, l1) (u2, l2)
-    -> UnitSteps m o (union u1 u2) (mergeLabel l1 l2).
+    -> UnitSteps m o (MF.union u1 u2) (mergeLabel l1 l2).
 
-Definition subtractKV {A : Type} 
-  (deceqA : forall (x y : A), sumbool (x = y) (x <> y))
-  (m1 m2 : Map A) : Map A := fun k => match m2 k, m1 k with
-  | Some v2, Some v1 => if deceqA v1 v2
-     then None
-     else Some v1
-  | _, m1k => m1k
-  end.
+Definition subtractKV {A : Type}
+  (deceqA : forall x y : A, sumbool (x = y) (x <> y))
+  (m1 m2 : M.t A) : M.t A :=
+    M.fold (fun k2 v2 m1' => match M.find k2 m1' with
+    | None => m1'
+    | Some v1 => if deceqA v1 v2 then 
+       M.remove k2 m1' else m1' 
+    end) m2 m1.
 
 Definition signIsEq : forall (l1 l2 : Typed SignT),
   sumbool (l1 = l2) (l1 <> l2).
@@ -112,8 +112,8 @@ Definition hide (l : LabelT) : LabelT := match l with
 
 Definition wellHidden (l : LabelT) (m : Modules) := match l with
   (rm, ds, cs) =>
-      NotOnDomain ds (getCmsMod m)
-    /\ NotOnDomain cs (getDmsMod m)
+      MF.NotOnDomain ds (getCmsMod m)
+    /\ MF.NotOnDomain cs (getDmsMod m)
   end.
 
 Inductive Step (m : Modules) (o u : RegsT) : LabelT -> Type :=
@@ -156,7 +156,7 @@ Section Decomposition.
     | UnitStepsUnion _ _ _ _ step1 step2 canCombine => 
       let (u1, l1) := Ts step1 in
       let (u2, l2) := Ts step2 in
-      (union u1 u2, mergeLabel l1 l2)
+      (MF.union u1 u2, mergeLabel l1 l2)
     end.
 
   Let Ts' {oImp nImp lImp} (step : Step imp oImp nImp lImp)
@@ -186,37 +186,37 @@ Section Decomposition.
   -> CanCombine (T step1) (T step2).
 
   Lemma canCombineLeft : forall {t u1 u2 l1 l2},
-    CanCombine t (union u1 u2, mergeLabel l1 l2)
+    CanCombine t (MF.union u1 u2, mergeLabel l1 l2)
   -> CanCombine t (u1, l1).
   Proof. intros.
   destruct l1 as [[rm1 ds1] cs1].
   destruct l2 as [[rm2 ds2] cs2].
   inversion H; clear H; subst. 
-  constructor; try (eapply Disj_union_1; eassumption).
+  constructor; try (eapply MF.Disj_union_1; eassumption).
   unfold bothNotRule in *. destruct rm1; intuition.
   Qed.
 
   Lemma canCombineRight : forall {t u1 u2 l1 l2},
-    CanCombine t (union u1 u2, mergeLabel l1 l2)
+    CanCombine t (MF.union u1 u2, mergeLabel l1 l2)
   -> CanCombine t (u2, l2).
   Proof. intros.
   destruct l1 as [[rm1 ds1] cs1].
   destruct l2 as [[rm2 ds2] cs2].
   inversion H; clear H; subst. 
-  constructor; try (eapply Disj_union_2; eassumption).
+  constructor; try (eapply MF.Disj_union_2; eassumption).
   unfold bothNotRule in *. destruct rm1; intuition.
   Qed.
 
   Lemma canCombineMerge : forall {t u1 u2 l1 l2},
     CanCombine t (u1, l1)
   -> CanCombine t (u2, l2)
-  -> CanCombine t (union u1 u2, mergeLabel l1 l2).
+  -> CanCombine t (MF.union u1 u2, mergeLabel l1 l2).
   Proof. intros. destruct t as [uL [[rmL csL] dsL]]. 
   destruct (mergeLabel l1 l2) as [[rm1 cs] ds] eqn:labeleqn.
   inversion H; inversion H0; inversion labeleqn; subst.
-  econstructor. apply Disj_union; assumption.
-  apply Disj_union; assumption.
-  apply Disj_union; assumption.
+  econstructor. apply MF.Disj_union; assumption.
+  apply MF.Disj_union; assumption.
+  apply MF.Disj_union; assumption.
   unfold bothNotRule in *; destruct rmL, rm2, rm4; intuition.
   Qed.  
 
@@ -225,7 +225,7 @@ Section Decomposition.
   Proof. 
    intros t1 t2 H;
    inversion H; clear H; subst; 
-   constructor; eauto using Disj_comm.
+   constructor; eauto using MF.Disj_comm.
    unfold bothNotRule in *.
    destruct rm1, rm2; intuition.
   Qed. 
@@ -275,8 +275,8 @@ Qed.
     destruct (Ts steps2) as [uSpec2 lSpec2].
    intuition. 
    unfold update in *.
-   fold (@union (Typed (fullType type))) in *.
-   rewrite <- union_assoc.
+   fold (@MF.union (Typed (fullType type))) in *.
+   rewrite <- MF.union_assoc.
    rewrite H3. admit. unfold equivalent in *. subst.
    admit.
    apply UnitStepsUnion. assumption. assumption.
